\documentclass[journal,12pt,twocolumn]{IEEEtran}

\usepackage{tfrupee}
\usepackage{enumitem}
\usepackage{amsmath}
\usepackage{amssymb}



\title{Assignment 2}
\author{Suraj kumar \\ \normalsize AI21BTECH11029 \\}
\begin{document}
\maketitle
\textbf{Question (9)} $\Rightarrow$ Solve the differential equation :
  \begin{align*}
  \frac{dy}{dx}=\frac{x+y+2}{2(x+y)-1}
  \end{align*}
  
\textbf{Solution}:
\begin{align}
let \hspace{10mm} &x+y=t
\end{align}
 differentiate (i) w.r.t to $x$
 \begin{align}
 	& 1+\frac{dy}{dx}=\frac{dt}{dx}\\
  	& \frac{dy}{dx}=\frac{dt}{dx}-1
 \end{align}
now substituting the value of $\frac{dy}{dx}$ in question
\begin{align}
	\frac{dt}{dx}-1&=\frac{t+2}{2t-1}\\
	\frac{dt}{dx}&=\frac{t+2}{2t-1}+1\\
	\frac{dt}{dx}&=\frac{t+2+2t-1}{2t-1}\\
	\frac{dt}{dx}&=\frac{3t+1}{2t-1}\\	
	\frac{2t-1}{3t+1}dt&=dx\\	
	\int \frac{2t-1}{3t+1}dt&=\int dx\\
	\int \left( \frac{2}{3}-\frac{5}{3(3t+1)} \right)dt&=\int dx\\
	\int \frac{2}{3}dt- \int \frac{5}{3(3t+1)}dt&=\int dx\\
	\frac{2}{3}\int dt-\frac{5}{3} \int \frac{1}{3t+1}dt&=\int dx\\
	\frac{2}{3} t-\frac{5}{3}\frac{\ln{3t+1}}{3}&=x+C_1\\
	\frac{2}{3} t-\frac{5(\ln{3t+1)}}{9}&=x+C_1
\end{align}
putting the value of t in equation $(15)$
\begin{align}
\frac{2}{3}(x+y)-\frac{5(\ln(3(x+y)+1)}{9}&=x+C_1
\end{align}
\end{document}